ok

SStructTT/SStruct/Runtime/Preservation1.lean
@@ -8,10 +8,67 @@ namespace Runtime
 open Dynamic
 variable {Srt : Type} [ord : SrtOrder Srt]
 
+def Pad (H1 H2 : Heap Srt) : Prop :=
+  ∃ H0, Contra H0 ∧ Finmap.Disjoint H1 H0 ∧ H2 = H1 ∪ H0
+
+lemma Pad.refl (H : Heap Srt) : Pad H H := by
+  exists ∅; and_intros
+  apply Contra.empty
+  apply Finmap.Disjoint.symm
+  apply Finmap.disjoint_empty
+  simp
+
+lemma Pad.insert (H : Heap Srt) l m s :
+    l ∉ H -> s ∈ ord.contra_set -> Pad H (H.insert l (m, s)) := by
+  intro h1 h2
+  exists Finmap.singleton l (m, s); and_intros
+  . intro x
+    if e: x = l then
+      subst_vars; simp
+      assumption
+    else
+      rw[<-Finmap.mem_singleton x l (m, s) (β := fun _ => Tm Srt × Srt)] at e
+      rw[Finmap.mem_iff] at e
+      split <;> try aesop
+  . rw[Finmap.Disjoint.eq_1]
+    intro x h0 h1
+    simp at h1; subst h1
+    contradiction
+  . apply Finmap.ext_lookup; intro x
+    if e: x = l then
+      subst_vars; simp[h1]
+    else
+      simp[e]
+      rw[Finmap.lookup_union_left_of_not_in]
+      intro h; simp at h
+      contradiction
+
+lemma Contra.union (H1 H2 : Heap Srt) : Contra H1 -> Contra H2 -> Contra (H1 ∪ H2) := by
+  intro ct1 ct2 x
+  replace ct1 := ct1 x
+  replace ct2 := ct2 x
+  split <;> try trivial
+  case h_1 heq =>
+    simp at heq
+    cases heq <;> aesop
+
+lemma Pad.contra (H1 H2 : Heap Srt) : Pad H1 H2 -> Contra H1 -> Contra H2 := by
+  intro pd c1
+  rcases pd with ⟨H0, ct, dsj, mrg⟩
+  rw[mrg]
+  apply Contra.union <;> assumption
+
+lemma Pad.split {H1 H2 H3 H3p : Heap Srt} :
+    Pad H3 H3p -> HMerge H1 H2 H3 ->
+    ∃ H1p H2p, Pad H1 H1p ∧ Pad H2 H2p ∧ HMerge H1p H2p H3p := by
+  sorry
+
 lemma Resolved.preservation1 {H1 H2 H3 H3' : Heap Srt} {a b c c' A} :
     HMerge H1 H2 H3 -> WR H2 ->
     [] ;; [] ;; H1 ⊢ a ▷ b ◁ c : A -> Step1 (H3, c) (H3', c') ->
-    ∃ H1', HMerge H1' H2 H3' ∧ [] ;; [] ;; H1' ⊢ a ▷ b ◁ c' : A := by
+    ∃ H1' H2',
+      HMerge H1' H2' H3' ∧ WR H2' ∧ Pad H2 H2' ∧
+      [] ;; [] ;; H1' ⊢ a ▷ b ◁ c' : A := by
   generalize e1: [] = Γ
   generalize e2: [] = Δ
   intro mrg0 wr2 ⟨er, rs, wr1⟩ st; induction er generalizing H1 H2 H3 H3' c c'
@@ -22,18 +79,9 @@ lemma Resolved.preservation1 {H1 H2 H3 H3' : Heap Srt} {a b c c' A} :
     case lam x rsx lwx =>
       cases st
       case alloc s l h vl =>
+        clear ihm
         cases vl
-        have ⟨h1, h2⟩ := mrg0.split_none h
-        have nfm := erm.nf; simp at nfm
-        have nfx := rsx.nf_preimage wr1 nfm
-        exists H1.insert l (x.lam s, s); and_intros
-        . apply mrg0.insert_left; assumption
-        . constructor
-          . apply Erased.lam_im <;> assumption
-          . apply Resolve.ptr
-            . assumption
-            . constructor <;> assumption
-          . apply wr1.insert_lam nfx
+        sorry
     case ptr =>
       cases st
       case alloc vl => cases vl
@@ -46,17 +94,45 @@ lemma Resolved.preservation1 {H1 H2 H3 H3' : Heap Srt} {a b c c' A} :
         have ⟨h1, h2⟩ := mrg0.split_none h
         have nfm := erm.nf; simp at nfm
         have nfx := rsx.nf_preimage wr1 nfm
-        exists H1.insert l (x.lam s, s); and_intros
-        . apply mrg0.insert_left; assumption
-        . constructor
-          . apply Erased.lam_ex <;> assumption
-          . apply Resolve.ptr
-            . assumption
-            . constructor <;> assumption
-          . apply wr1.insert_lam nfx
+        if h3: s ∈ ord.contra_set then
+          replace lwx := lwx h3
+          exists H1.insert l (x.lam s, s), H2.insert l (x.lam s, s); and_intros
+          . apply mrg0.insert_contra
+            assumption
+          . apply wr2.insert_lam nfx
+          . apply Pad.insert
+            simp[<-Finmap.mem_keys,h2]
+            assumption
+          . constructor
+            . apply Erased.lam_ex <;> assumption
+            . apply Resolve.ptr
+              . unfold HLookup
+                simp[h3]; aesop
+              . constructor
+                intro; apply lwx.insert; assumption
+                sorry
+            . apply wr1.insert_lam nfx
+        else
+          exists H1.insert l (x.lam s, s), H2; and_intros
+          . apply mrg0.insert_left
+            assumption
+            assumption
+          . assumption
+          . apply Pad.refl
+          . constructor
+            . apply Erased.lam_ex <;> assumption
+            . apply Resolve.ptr
+              pick_goal 2
+              . constructor <;> assumption
+              . unfold HLookup
+                simp[h3,Heap.erase_insert,h1]
+            . apply wr1.insert_lam nfx
     case ptr =>
       cases st
       case alloc vl => cases vl
+  all_goals sorry
+
+/-
   case app_im erm tyn ihm =>
     subst_vars; cases rs
     case app mrg1 rsm rsn =>
@@ -370,3 +446,30 @@ lemma Resolved.preservation1' {H1 H2 H3 H3' : Heap Srt} {a b c c' A} :
     replace ⟨H1, mrg1, rs1⟩ := ih rfl mrg wr rs
     have ⟨H2, mrg2, st2⟩ := rs1.preservation1 mrg1 wr st
     exists H2
+
+-/
+
+lemma Resolved.preservation1X {H1 H2 : Heap Srt} {a b c c' A} :
+    [] ;; [] ;; H1 ⊢ a ▷ b ◁ c : A -> Step1 (H1, c) (H2, c') ->
+    [] ;; [] ;; H2 ⊢ a ▷ b ◁ c' : A := by
+  intro rsm st
+  have ⟨H0, mrg, ct⟩ := HMerge.exists_self_contra H1
+  have ⟨_, _, wr⟩ := rsm
+  have wr0 := mrg.sym.split_wr' wr
+  have ⟨H1', H2', mrg', wr', pd, rsm'⟩ := rsm.preservation1 mrg wr0 st
+  have ct := pd.contra _ _ ct
+  sorry
+  -- have e := mrg'.sym.contra ct; subst e
+  -- assumption
+
+lemma Resolved.preservation1' {H1 H2 : Heap Srt} {a b c c' A} :
+    [] ;; [] ;; H1 ⊢ a ▷ b ◁ c : A -> Red1 (H1, c) (H2, c') ->
+    [] ;; [] ;; H2 ⊢ a ▷ b ◁ c' : A := by
+  generalize e: (H2, c') = t
+  intro rs rd; induction rd generalizing H2 a b c' A
+  case R => cases e; assumption
+  case SE y z rd st ih =>
+    subst_vars
+    rcases y with ⟨H2, c'⟩
+    replace rs' := ih rfl rs
+    apply rs'.preservation1X st
